src/lib/GPU.Math.fsti
@@ -1,0 +1,20 @@
+module GPU.Math
+
+let rec log2 (n:pos) : GTot (r:nat{r < n}) =
+  if n = 1 then 0 else 1 + log2 (n / 2)
+
+val pow_log_lemma (n: nat)
+: Lemma (log2 (pow2 n) == n)
+  [SMTPat (log2 (pow2 n))]
+
+let min (a b: int) : GTot int =
+  if a < b then a else b
+
+(* x is a multiple of 2^i *)
+let div_pow2 (i x : nat) : GTot bool =
+  (x % pow2 i) = 0
+
+val div_pow2_lemma (i j tid: nat):
+  Lemma
+    (requires i < j)
+    (ensures (div_pow2 j tid) ==> (div_pow2 i tid))
